<?xml version="1.0" encoding="utf-8" ?>
<rdf:RDF xmlns:rdf="http://www.w3.org/1999/02/22-rdf-syntax-ns#"
         xmlns:owl="http://www.w3.org/2002/07/owl#"
         xmlns:xsd="http://www.w3.org/2001/XMLSchema#"
         xmlns:dc="http://purl.org/dc/elements/1.1/"
         xmlns:dcterms="http://purl.org/dc/terms/"
         xmlns:rdfs="http://www.w3.org/2000/01/rdf-schema#"
         xmlns:skos="http://www.w3.org/2004/02/skos/core#"
         xmlns:schema="http://schema.org/"
         xmlns:geolink="http://schema.geolink.org/1.0/base/main#"
         xmlns:gdx="https://geodex.org/voc/">

  <owl:Ontology rdf:about="gdx:">
    <dc:description>Schema.org extension for a Information Resource Service</dc:description>
    <dc:title>Information Resource Service Vocabulary</dc:title>
    <dc:creator>EarthCube Registry Working Group</dc:creator>
    <dcterms:issued rdf:datatype="xsd:date">2017-10-16</dcterms:issued>
    <owl:versionInfo>0.1.0</owl:versionInfo>
  </owl:Ontology>

  <!-- RULES
    1. If gdx:ResearchRepositoryService schema:provider <resource>,
       then there must be a Role
       where performedBy is <resource>
       and roleType is gdx:RoleType-ResearchRepositoryServiceProvider
  -->


  <owl:Class rdf:about="gdx:ResearchRepositoryService">
    <rdfs:subClassOf rdf:resource="schema:Service"/>
    <rdfs:subClassOf>
      <owl:Restriction>
        <owl:onProperty rdf:resource="schema:name"/>
        <owl:cardinality rdf:datatype="xsd:nonNegativeInteger">1</owl:cardinality>
      </owl:Restriction>
    </rdfs:subClassOf>
    <rdfs:subClassOf>
      <owl:Restriction>
        <owl:onProperty rdf:resource="schema:url"/>
        <owl:cardinality rdf:datatype="xsd:nonNegativeInteger">1</owl:cardinality>
      </owl:Restriction>
    </rdfs:subClassOf>
    <rdfs:subClassOf>
      <owl:Restriction>
        <owl:onProperty rdf:resource="schema:description"/>
        <owl:maxCardinality rdf:datatype="xsd:nonNegativeInteger">1</owl:maxCardinality>
      </owl:Restriction>
    </rdfs:subClassOf>
    <rdfs:subClassOf>
      <owl:Restriction>
        <owl:onProperty rdf:resource="gdx:hasResourceCatalog"/>
        <owl:minCardinality rdf:datatype="xsd:nonNegativeInteger">1</owl:minCardinality>
      </owl:Restriction>
    </rdfs:subClassOf>
    <rdfs:subClassOf>
      <owl:Restriction>
        <owl:onProperty rdf:resource="schema:provider"/>
        <owl:someValuesFrom rdf:resource="gdx:Institution"/>
        <owl:minCardinality rdf:datatype="xsd:nonNegativeInteger">1</owl:minCardinality>
      </owl:Restriction>
    </rdfs:subClassOf>
    <rdfs:subClassOf>
      <owl:Restriction>
        <owl:onProperty rdf:resource="gdx:supportService"/>
        <owl:minCardinality rdf:datatype="xsd:nonNegativeInteger">1</owl:minCardinality>
      </owl:Restriction>
    </rdfs:subClassOf>
    <rdfs:subClassOf>
      <owl:Restriction>
        <owl:onProperty rdf:resource="gdx:searchService"/>
        <owl:minCardinality rdf:datatype="xsd:nonNegativeInteger">1</owl:minCardinality>
      </owl:Restriction>
    </rdfs:subClassOf>
    <rdfs:subClassOf>
      <owl:Restriction>
        <owl:onProperty rdf:resource="gdx:subjectArea"/>
        <owl:minCardinality rdf:datatype="xsd:nonNegativeInteger">1</owl:minCardinality>
      </owl:Restriction>
    </rdfs:subClassOf>
    <rdfs:isDefinedBy rdf:resource="gdx:"/>
    <rdfs:label xml:lang="en">Research Repository Service</rdfs:label>
    <rdfs:comment xml:lang="en">A service providing access to products developed from research activities such as data, software and other research outputs.</rdfs:comment>
  </owl:Class>

  <owl:ObjectProperty rdf:resource="gdx:hasResourceCatalog">
    <rdf:type rdf:resource="rdf:Property"/>
    <rdfs:subPropertyOf rdf:resource="schema:hasOfferCatalog"/>
    <rdfs:isDefinedBy rdf:resource="gdx:"/>
    <rdfs:domain rdf:resource="gdx:ResearchRepositoryService"/>
    <rdfs:range rdf:resource="gdx:ResearchResourceCatalog"/>
    <rdfs:label xml:lang="en">hasResourceCatalog</rdfs:label>
    <rdfs:comment xml:lang="en">Indicates an OfferCatalog listing of CreativeWorks for this Service.</rdfs:comment>
  </owl:ObjectProperty>

  <owl:Class rdf:about="gdx:ResearchResourceCatalog">
    <rdfs:subClassOf rdf:resource="schema:OfferCatalog"/>
    <rdfs:subClassOf>
      <owl:Restriction>
        <owl:onProperty rdf:resource="schema:itemListElement"/>
        <owl:allValuesFrom rdf:resource="schema:CreativeWork"/>
      </owl:Restriction>
    </rdfs:subClassOf>
    <rdfs:isDefinedBy rdf:resource="gdx:"/>
    <rdfs:label xml:lang="en">Research Repository Service</rdfs:label>
    <rdfs:comment xml:lang="en">A service providing access to products developed from research activities such as data, software and other research outputs.</rdfs:comment>
  </owl:Class>

  <owl:ObjectProperty rdf:about="gdx:supportService">
    <rdf:type rdf:resource="rdf:Property"/>
    <rdfs:subPropertyOf rdf:resource="schema:availableChannel"/>
    <rdfs:isDefinedBy rdf:resource="gdx:"/>
    <rdfs:domain rdf:resource="gdx:ResearchRepositoryService"/>
    <rdfs:range rdf:resource="schema:ServiceChannel"/>
    <rdfs:label xml:lang="en">supportService</rdfs:label>
    <rdfs:comment xml:lang="en">Provides a channel for contacting support for a research resource respository.</rdfs:comment>
  </owl:ObjectProperty>

  <owl:ObjectProperty rdf:about="gdx:searchService">
    <rdf:type rdf:resource="rdf:Property"/>
    <rdfs:subPropertyOf rdf:resource="schema:availableChannel"/>
    <rdfs:isDefinedBy rdf:resource="gdx:"/>
    <rdfs:domain rdf:resource="gdx:ResearchRepositoryService"/>
    <rdfs:range rdf:resource="schema:ServiceChannel"/>
    <rdfs:label xml:lang="en">searchService</rdfs:label>
    <rdfs:comment xml:lang="en">Provides a channel for searching for research resources at a respository.</rdfs:comment>
  </owl:ObjectProperty>

  <owl:ObjectProperty rdf:about="gdx:submissionService">
    <rdf:type rdf:resource="rdf:Property"/>
    <rdfs:subPropertyOf rdf:resource="schema:availableChannel"/>
    <rdfs:isDefinedBy rdf:resource="gdx:"/>
    <rdfs:domain rdf:resource="gdx:ResearchRepositoryService"/>
    <rdfs:range rdf:resource="schema:ServiceChannel"/>
    <rdfs:label xml:lang="en">submissionService</rdfs:label>
    <rdfs:comment xml:lang="en">Provides a channel for submitting research resources to a respository.</rdfs:comment>
  </owl:ObjectProperty>

  <owl:ObjectProperty rdf:about="gdx:syndicationService">
    <rdf:type rdf:resource="rdf:Property"/>
    <rdfs:subPropertyOf rdf:resource="schema:availableChannel"/>
    <rdfs:isDefinedBy rdf:resource="gdx:"/>
    <rdfs:domain rdf:resource="gdx:ResearchRepositoryService"/>
    <rdfs:range rdf:resource="schema:ServiceChannel"/>
    <rdfs:label xml:lang="en">syndicationService</rdfs:label>
    <rdfs:comment xml:lang="en">Provides a channel for alerting the user community of updates at a repository.</rdfs:comment>
  </owl:ObjectProperty>

  <owl:DatatypeProperty rdf:about="gdx:serviceEmail">
    <rdf:type rdf:resource="rdf:Property"/>
    <skos:subPropertyOf rdf:resource="schema:email"/>
    <rdfs:isDefinedBy rdf:resource="gdx:"/>
    <rdfs:domain rdf:resource="schema:ServiceChannel"/>
    <rdfs:range rdf:resource="schema:Text"/>
    <rdfs:label xml:lang="en">serviceEmail</rdfs:label>
    <rdfs:comment xml:lang="en">Provides a channel for contacting support for a research resource respository.</rdfs:comment>
  </owl:DatatypeProperty>

  <owl:ObjectProperty rdf:about="gdx:subjectArea">
    <rdf:type rdf:resource="rdf:Property"/>
    <skos:closeMatch rdf:resource="schema:keywords"/>
    <rdfs:isDefinedBy rdf:resource="gdx:"/>
    <rdfs:domain rdf:resource="gdx:ResearchRepositoryService"/>
    <rdfs:range rdf:resource="gdx:SubjectArea"/>
    <rdfs:label xml:lang="en">subjectArea</rdfs:label>
    <rdfs:comment xml:lang="en">The disciplinary focus of the repository.</rdfs:comment>
  </owl:ObjectProperty>

  <owl:Class rdf:about="gdx:SubjectArea">
    <rdfs:subClassOf rdf:resource="schema:Thing"/>
    <rdfs:subClassOf>
      <owl:Restriction>
        <owl:onProperty rdf:resource="schema:name"/>
        <owl:cardinality rdf:datatype="xsd:nonNegativeInteger">1</owl:cardinality>
      </owl:Restriction>
    </rdfs:subClassOf>
    <rdfs:isDefinedBy rdf:resource="gdx:"/>
    <rdfs:label xml:lang="en">Subject Area</rdfs:label>
    <rdfs:comment xml:lang="en">A disciplinary focus for the contents of the respository.</rdfs:comment>
  </owl:Class>

  <owl:ObjectProperty rdf:about="gdx:providesRole">
    <rdf:type rdf:resource="rdf:Property"/>
    <rdfs:isDefinedBy rdf:resource="gdx:"/>
    <rdfs:domain rdf:resource="schema:Thing"/>
    <rdfs:range rdf:resource="gdx:Role"/>
    <rdfs:label xml:lang="en">providesRole</rdfs:label>
    <rdfs:comment xml:lang="en">Provides the opportunity for an agent to serve in a specific role.</rdfs:comment>
  </owl:ObjectProperty>

  <owl:ObjectProperty rdf:about="gdx:performsRoleFor">
    <rdf:type rdf:resource="rdf:Property"/>
    <owl:inverseOf rdf:resource="gdx:providesRole"/>
    <rdfs:isDefinedBy rdf:resource="gdx:"/>
    <rdfs:domain rdf:resource="gdx:Role"/>
    <rdfs:range rdf:resource="schema:Thing"/>
    <rdfs:label xml:lang="en">performsRoleFor</rdfs:label>
    <rdfs:comment xml:lang="en">An Agent performing a specific type of role.</rdfs:comment>
  </owl:ObjectProperty>

  <owl:Class rdf:about="gdx:Role">
    <rdfs:subClassOf rdf:resource="schema:Thing"/>
    <skos:closeMatch rdf:resource="geolink:Participant"/>
    <rdfs:subClassOf>
      <owl:Restriction>
        <owl:onProperty rdf:resource="gdx:performedBy"/>
        <owl:cardinality rdf:datatype="xsd:nonNegativeInteger">1</owl:cardinality>
      </owl:Restriction>
    </rdfs:subClassOf>
    <rdfs:subClassOf>
      <owl:Restriction>
        <owl:onProperty rdf:resource="gdx:roleType"/>
        <owl:cardinality rdf:datatype="xsd:nonNegativeInteger">1</owl:cardinality>
      </owl:Restriction>
    </rdfs:subClassOf>
    <rdfs:isDefinedBy rdf:resource="gdx:"/>
    <rdfs:label xml:lang="en">Agent Role</rdfs:label>
    <rdfs:comment xml:lang="en">A single role performed by a single Agent.</rdfs:comment>
  </owl:Class>

  <owl:ObjectProperty rdf:about="gdx:performedBy">
    <rdf:type rdf:resource="rdf:Property"/>
    <rdfs:isDefinedBy rdf:resource="gdx:"/>
    <rdfs:domain rdf:resource="gdx:Role"/>
    <rdfs:range rdf:resource="gdx:Agent"/>
    <rdfs:label xml:lang="en">performedBy</rdfs:label>
    <rdfs:comment xml:lang="en">A role performed by a specific Agent.</rdfs:comment>
  </owl:ObjectProperty>

  <owl:ObjectProperty rdf:about="gdx:roleType">
    <rdf:type rdf:resource="rdf:Property"/>
    <rdfs:subPropertyOf rdf:resource="schema:additionalType"/>
    <rdfs:isDefinedBy rdf:resource="gdx:"/>
    <rdfs:domain rdf:resource="gdx:Role"/>
    <rdfs:range rdf:resource="gdx:RoleType"/>
    <rdfs:label xml:lang="en">roleType</rdfs:label>
    <rdfs:comment xml:lang="en">The type of role performed by an Agent.</rdfs:comment>
  </owl:ObjectProperty>

  <owl:Class rdf:about="gdx:Agent">
    <rdfs:subClassOf rdf:resource="schema:Thing"/>
    <skos:narrowMatch rdf:resource="schema:Organization"/>
    <skos:narrowMatch rdf:resource="schema:Person"/>
    <skos:narrowMatch rdf:resource="geolink:Organization"/>
    <skos:narrowMatch rdf:resource="geolink:Person"/>
    <rdfs:isDefinedBy rdf:resource="gdx:"/>
    <rdfs:label xml:lang="en">Agent</rdfs:label>
    <rdfs:comment xml:lang="en">A person or organization that performs a specific role for another Agent.</rdfs:comment>
  </owl:Class>

  <owl:Class rdf:about="gdx:RoleType">
    <rdfs:subClassOf rdf:resource="schema:Enumeration"/>
    <skos:exactMatch rdf:resource="geolink:RoleType"/>
    <rdfs:isDefinedBy rdf:resource="gdx:"/>
    <rdfs:label xml:lang="en">Agent Role Type</rdfs:label>
    <rdfs:comment xml:lang="en">An enumeration of types of Roles that can be performed by an Agent.</rdfs:comment>
  </owl:Class>

  <owl:namedIndividual rdf:about="gdx:RoleType-ContactPoint">
    <rdf:type rdf:resource="gdx:RoleType"/>
    <skos:closeMatch rdf:resource="schema:ContactPoint"/>
    <rdfs:isDefinedBy rdf:resource="gdx:"/>
    <rdfs:label xml:lang="en">Role: Point of Contact</rdfs:label>
    <rdfs:comment xml:lang="en">The point-of-contact.</rdfs:comment>
  </owl:namedIndividual>

  <owl:namedIndividual rdf:about="gdx:RoleType-ResearchRepositoryServiceProvider">
    <rdf:type rdf:resource="gdx:RoleType"/>
    <rdfs:isDefinedBy rdf:resource="gdx:"/>
    <rdfs:label xml:lang="en">Role: Provider</rdfs:label>
    <rdfs:comment xml:lang="en">The agent acting as the provider of the services for a Research Resource Repository.</rdfs:comment>
  </owl:namedIndividual>

  <owl:namedIndividual rdf:about="gdx:ResearchRepositoryServiceRoleType-FundingSource">
    <rdf:type rdf:resource="gdx:RoleType"/>
    <rdfs:isDefinedBy rdf:resource="gdx:"/>
    <rdfs:label xml:lang="en">Role: Funding Source</rdfs:label>
    <rdfs:comment xml:lang="en">An agent supplying funding for the Research Resource Repository. RDF resources for funding agencies can be found at Crossref (https://www.crossref.org/services/funder-registry/) through its Fundref project. As en example, the National Science Foundation has resource IRI 'http://dx.doi.org/10.13039/100000001' and the GEO directorate of NSF has resource IRI 'http://dx.doi.org/10.13039/100000085'. These IRIs can be used as the Agent for an Role through the 'gdx:performedBy' predicate.</rdfs:comment>
    <rdfs:seeAlso rdf:datatype="xsd:anyURI">https://www.crossref.org/services/funder-registry/</rdfs:seeAlso>
  </owl:namedIndividual>

  <owl:namedIndividual rdf:about="gdx:ResearchRepositoryServiceRoleType-Sponsor">
    <rdf:type rdf:resource="gdx:RoleType"/>
    <rdfs:isDefinedBy rdf:resource="gdx:"/>
    <rdfs:label xml:lang="en">Role: Sponsor</rdfs:label>
    <rdfs:comment xml:lang="en">An agent sponsoring the Research Resource Repository.</rdfs:comment>
  </owl:namedIndividual>

  <owl:namedIndividual rdf:about="gdx:ResearchRepositoryServiceRoleType-TechnicalServiceProvider">
    <rdf:type rdf:resource="gdx:RoleType"/>
    <rdfs:isDefinedBy rdf:resource="gdx:"/>
    <rdfs:label xml:lang="en">Role: Technical Service Provider</rdfs:label>
    <rdfs:comment xml:lang="en">An agent providing technical resources to the main Information Resource Repository.</rdfs:comment>
  </owl:namedIndividual>

  <owl:Class rdf:about="gdx:Institution">
    <rdfs:subClassOf rdf:resource="gdx:Agent"/>
    <skos:exactMatch rdf:resource="schema:Organization"/>
    <skos:exactMatch rdf:resource="geolink:Organization"/>
    <rdfs:subClassOf>
      <owl:Restriction>
        <owl:onProperty rdf:resource="schema:legalName"/>
        <owl:cardinality rdf:datatype="xsd:nonNegativeInteger">1</owl:cardinality>
      </owl:Restriction>
    </rdfs:subClassOf>
    <rdfs:isDefinedBy rdf:resource="gdx:"/>
    <rdfs:label xml:lang="en">Institution</rdfs:label>
    <rdfs:comment xml:lang="en">An organization that normally should continue to exist beyond the scope of the Research Resource repository. This institution is responsible for a specific role for the respository.</rdfs:comment>
  </owl:Class>

  <owl:ObjectProperty rdf:about="gdx:followsProtocol">
    <rdf:type rdf:resource="rdf:Property"/>
    <rdfs:isDefinedBy rdf:resource="gdx:"/>
    <rdfs:domain>
      <owl:Class>
        <owl:unionOf rdf:parseType="Collection">
          <rdf:Description rdf:about="gdx:ResearchRepositoryService"/>
          <rdf:Description rdf:about="schema:CreativeWork"/>
        </owl:unionOf>
      </owl:Class>
    </rdfs:domain>
    <rdfs:range rdf:resource="gdx:Protocol"/>
    <rdfs:label xml:lang="en">followsProtocol</rdfs:label>
    <rdfs:comment xml:lang="en">Defines a Protocol to interacting with either the repository or with specific offerings of the repository.</rdfs:comment>
  </owl:ObjectProperty>

  <owl:Class rdf:about="gdx:Protocol">
    <rdfs:subClassOf rdf:resource="schema:DigitalDocument"/>
    <rdfs:subClassOf>
      <owl:Restriction>
        <owl:onProperty rdf:resource="schema:name"/>
        <owl:cardinality rdf:datatype="xsd:nonNegativeInteger">1</owl:cardinality>
      </owl:Restriction>
    </rdfs:subClassOf>
    <rdfs:subClassOf>
      <owl:Restriction>
        <owl:onProperty rdf:resource="schema:url"/>
        <owl:cardinality rdf:datatype="xsd:nonNegativeInteger">1</owl:cardinality>
      </owl:Restriction>
    </rdfs:subClassOf>
    <rdfs:subClassOf>
      <owl:Restriction>
        <owl:onProperty rdf:resource="gdx:protocolType"/>
        <owl:cardinality rdf:datatype="xsd:nonNegativeInteger">1</owl:cardinality>
      </owl:Restriction>
    </rdfs:subClassOf>
    <rdfs:isDefinedBy rdf:resource="gdx:"/>
    <rdfs:label xml:lang="en">Protocol</rdfs:label>
    <rdfs:comment xml:lang="en">Digital document explaining the expectations for interacting with the repository or its resources.</rdfs:comment>
  </owl:Class>

  <owl:ObjectProperty rdf:about="gdx:protocolType">
    <rdf:type rdf:resource="rdf:Property"/>
    <rdfs:subPropertyOf rdf:resource="schema:additionalType"/>
    <rdfs:isDefinedBy rdf:resource="gdx:"/>
    <rdfs:domain rdf:resource="gdx:Protocol"/>
    <rdfs:range rdf:resource="gdx:ProtocolType"/>
    <rdfs:label xml:lang="en">protocolType</rdfs:label>
    <rdfs:comment xml:lang="en">Specifies the type of Protocol.</rdfs:comment>
  </owl:ObjectProperty>

  <owl:Class rdf:about="gdx:ProtocolType">
    <rdfs:subClassOf rdf:resource="schema:Enumeration"/>
    <rdfs:isDefinedBy rdf:resource="gdx:"/>
    <rdfs:label xml:lang="en">Protocol Type</rdfs:label>
    <rdfs:comment xml:lang="en">Identifies the type of Protocol.</rdfs:comment>
  </owl:Class>

  <owl:namedIndividual rdf:about="gdx:ProtocolType-Access">
    <rdf:type rdf:resource="gdx:protocolType"/>
    <rdfs:isDefinedBy rdf:resource="gdx:"/>
    <rdfs:label xml:lang="en">Access Protocol</rdfs:comment>
    <rdfs:comment xml:lang="en">An access regulation.</rdfs:comment>
  </owl:namedIndividual>

  <owl:namedIndividual rdf:about="gdx:ProtocolType-PreservationPolicy">
    <rdf:type rdf:resource="gdx:protocolType"/>
    <rdfs:isDefinedBy rdf:resource="gdx:"/>
    <rdfs:label xml:lang="en">Preservation Policy</rdfs:comment>
    <rdfs:comment xml:lang="en">A policy describing a preservation protocol.</rdfs:comment>
  </owl:namedIndividual>

  <owl:namedIndividual rdf:about="gdx:ProtocolType-ResourceSubmissionPolicy">
    <rdf:type rdf:resource="gdx:protocolType"/>
    <rdfs:isDefinedBy rdf:resource="gdx:"/>
    <rdfs:label xml:lang="en">Resource Submission Policy</rdfs:comment>
    <rdfs:comment xml:lang="en">A policy describing the protocols for submitting resources to the repository.</rdfs:comment>
  </owl:namedIndividual>

  <owl:namedIndividual rdf:about="gdx:ProtocolType-TermsOfUse">
    <rdf:type rdf:resource="gdx:protocolType"/>
    <rdfs:isDefinedBy rdf:resource="gdx:"/>
    <rdfs:label xml:lang="en">Terms of Use</rdfs:comment>
    <rdfs:comment xml:lang="en">A policy describing the Terms of Use.</rdfs:comment>
  </owl:namedIndividual>

  <owl:namedIndividual rdf:about="gdx:ProtocolType-License">
    <rdf:type rdf:resource="gdx:protocolType"/>
    <rdfs:isDefinedBy rdf:resource="gdx:"/>
    <rdfs:label xml:lang="en">License</rdfs:comment>
    <rdfs:comment xml:lang="en">An applicable license.</rdfs:comment>
  </owl:namedIndividual>

