@prefix owl: <http://www.w3.org/2002/07/owl#> .
@prefix dc11: <http://purl.org/dc/elements/1.1/> .
@prefix dc: <http://purl.org/dc/terms/> .
@prefix xsd: <http://www.w3.org/2001/XMLSchema#> .
@prefix rdfs: <http://www.w3.org/2000/01/rdf-schema#> .
@prefix schema: <http://schema.org/> .
@prefix skos: <http://www.w3.org/2004/02/skos/core#> .

<gdx:>
  a owl:Ontology ;
  dc11:description "Schema.org extension for a Information Resource Service"@en-US ;
  dc11:title "Research Repository Service Vocabulary"@en-US ;
  dc11:creator "EarthCube Registry Working Group"@en-US ;
  dc:source "https://github.com/earthcubearchitecture-project418"^^xsd:anyURI ;
  dc:issued "2017-11-27"^^xsd:date ;
  owl:versionInfo "0.8.0" .

<gdx:ResearchRepositoryService>
  a owl:Class ;
  rdfs:subClassOf schema:Service, [
    a owl:Restriction ;
    owl:onProperty schema:name ;
    owl:cardinality "1"^^xsd:nonNegativeInteger
  ], [
    a owl:Restriction ;
    owl:onProperty schema:url ;
    owl:cardinality "1"^^xsd:nonNegativeInteger
  ], [
    a owl:Restriction ;
    owl:onProperty schema:description ;
    owl:maxCardinality "1"^^xsd:nonNegativeInteger
  ], [
    a owl:Restriction ;
    owl:onProperty schema:provider ;
    owl:minCardinality "1"^^xsd:nonNegativeInteger
  ] ;
  rdfs:isDefinedBy <gdx:> ;
  rdfs:label "Research Repository Service"@en-US ;
  rdfs:comment "A service providing access to products developed from research activities such as data, software and other research outputs."@en-US .

<gdx:SearchService>
  a owl:namedIndividual, schema:Service ;
  skos:related schema:SearchAction ;
  rdfs:isDefinedBy <gdx:> ;
  rdfs:label "Search Service"@en-US ;
  rdfs:comment "A service provided for searching the resource catalog."@en-US .

<gdx:SubmissionService>
  a owl:namedIndividual, schema:Service ;
  skos:related schema:CreateAction ;
  rdfs:isDefinedBy <gdx:> ;
  rdfs:label "Submssions Service"@en-US ;
  rdfs:comment "A service provided for submitting resources to the catalog."@en-US .

<gdx:SyndicationService>
  a owl:namedIndividual, schema:Service ;
  skos:related schema:ConsumeAction ;
  rdfs:isDefinedBy <gdx:> ;
  rdfs:label "Syndication Service"@en-US ;
  rdfs:comment "A service provided for syndicating resources from the catalog."@en-US .

<gdx:Protocol-Access>
  a owl:namedIndividual, schema:DigitalDocument ;
  rdfs:isDefinedBy <gdx:> ;
  rdfs:label "Access Protocol"@en-US ;
  rdfs:comment "An access regulation."@en-US .

<gdx:Protocol-PreservationPolicy>
  a owl:namedIndividual, schema:DigitalDocument ;
  rdfs:isDefinedBy <gdx:> ;
  rdfs:label "Preservation Policy"@en-US ;
  rdfs:comment "A policy describing a preservation protocol."@en-US .

<gdx:Protocol-ResourceSubmissionPolicy>
  a owl:namedIndividual, schema:DigitalDocument ;
  rdfs:isDefinedBy <gdx:> ;
  rdfs:label "Resource Submission Policy"@en-US ;
  rdfs:comment "A policy describing the protocols for submitting resources to the repository."@en-US .

<gdx:Protocol-TermsOfUse>
  a owl:namedIndividual, schema:DigitalDocument ;
  rdfs:isDefinedBy <gdx:> ;
  rdfs:label "Terms of Use"@en-US ;
  rdfs:comment "A policy describing the Terms of Use."@en-US .

<gdx:Protocol-License>
  a owl:namedIndividual, schema:DigitalDocument ;
  rdfs:isDefinedBy <gdx:> ;
  rdfs:label "License"@en-US ;
  rdfs:comment "An applicable license."@en-US .

<gdx:SitemapXML>
  a owl:namedIndividual, schema:DigitalDocument ;
  skos:related <gdx:SyndicationService> ;
  rdfs:isDefinedBy <gdx:> ;
  rdfs:label "Sitemap XML"@en-US ;
  rdfs:comment "A sitemap.xml file for a website that exposes URLs that should be indexed by a search engine harvester. A sitemap.xml file is one way to provide access to all resources offered by the catalog."@en-US .

<gdx:ResearchResourceTypes>
  a owl:namedIndividual, schema:OfferCatalog ;
  rdfs:isDefinedBy <gdx:> ;
  skos:related schema:CreativeWork ;
  rdfs:label "Research Resource Types"@en-US ;
  rdfs:comment "A list of research resource types (aka schema:CreativeWork) offered by a ResearchRepositoryService."@en-US .

<gdx:OutreachActivities>
  a owl:namedIndividual, schema:OfferCatalog ;
  rdfs:isDefinedBy <gdx:> ;
  rdfs:label "Outreach Activity"@en-US ;
  rdfs:comment "A list of outreach activities offered by a ResearchRepositoryService."@en-US .

<gdx:OutreachActivity-Training>
  a owl:namedIndividual, schema:Action ;
  rdfs:isDefinedBy <gdx:> ;
  rdfs:label "Training Outreach Activity"@en-US ;
  rdfs:comment "A training activity offered by a ResearchRepositoryService."@en-US .

<gdx:OutreachActivity-UserWorkshop>
  a owl:namedIndividual, schema:Action ;
  rdfs:isDefinedBy <gdx:> ;
  rdfs:label "User Workshop Outreach Activity"@en-US ;
  rdfs:comment "A user workshop activity offered by a ResearchRepositoryService."@en-US .

<gdx:OutreachActivity-UserSupport>
  a owl:namedIndividual, schema:Action ;
  rdfs:isDefinedBy <gdx:> ;
  rdfs:label "User Support Outreach Activity"@en-US ;
  rdfs:comment "A user support activity offered by a ResearchRepositoryService."@en-US .

<gdx:fundedBy>
  a owl:ObjectProperty, rdf:Property ;
  rdfs:isDefinedBy <gdx:> ;
  rdfs:label "fundedBy"@en-US ;
  rdfs:comment "A funding award that facilitated the generation of a creative work."@en-US ;
  rdfs:domain schema:CreativeWork ;
  rdfs:range schema:Offer .
