@prefix owl: <http://www.w3.org/2002/07/owl#> .
@prefix dc11: <http://purl.org/dc/elements/1.1/> .
@prefix dc: <http://purl.org/dc/terms/> .
@prefix xsd: <http://www.w3.org/2001/XMLSchema#> .
@prefix rdfs: <http://www.w3.org/2000/01/rdf-schema#> .
@prefix schema: <http://schema.org/> .
@prefix rdf: <http://www.w3.org/1999/02/22-rdf-syntax-ns#> .

<gdx:>
  a owl:Ontology ;
  dc11:description ">Schema.org extension for a Information Resource Service"@en-US ;
  dc11:title ">Research Repository Service Vocabulary"@en-US ;
  dc11:creator "EarthCube Registry Working Group"@en-US ;
  dc:source "https://github.com/earthcubearchitecture-project418"^^xsd:anyURI ;
  dc:issued "2017-10-16"^^xsd:date ;
  owl:versionInfo "0.7.0" .

<gdx:ResearchRepositoryService>
  a owl:Class ;
  rdfs:subClassOf schema:Service, [
    a owl:Restriction ;
    owl:onProperty schema:name ;
    owl:cardinality "1"^^xsd:nonNegativeInteger
  ], [
    a owl:Restriction ;
    owl:onProperty schema:url ;
    owl:cardinality "1"^^xsd:nonNegativeInteger
  ], [
    a owl:Restriction ;
    owl:onProperty schema:description ;
    owl:maxCardinality "1"^^xsd:nonNegativeInteger
  ], [
    a owl:Restriction ;
    owl:onProperty <gdx:hasResourceCatalog> ;
    owl:minCardinality "1"^^xsd:nonNegativeInteger
  ], [
    a owl:Restriction ;
    owl:onProperty schema:provider ;
    owl:minCardinality "1"^^xsd:nonNegativeInteger
  ] ;
  rdfs:isDefinedBy <gdx:> ;
  rdfs:label "Research Repository Service"@en-US ;
  rdfs:comment "A service providing access to products developed from research activities such as data, software and other research outputs."@en-US .

<gdx:hasResourceCatalog>
  a owl:ObjectProperty, rdf:Property ;
  rdfs:subPropertyOf schema:hasOfferCatalog ;
  rdfs:isDefinedBy <gdx:> ;
  rdfs:domain <gdx:ResearchRepositoryService> ;
  rdfs:range <gdx:ResearchResourceCatalog> ;
  rdfs:label "hasResourceCatalog"@en-US ;
  rdfs:comment "Indicates an OfferCatalog listing of CreativeWorks for this Service."@en-US .

<gdx:ResearchResourceCatalog>
  a owl:Class ;
  rdfs:subClassOf schema:OfferCatalog, [
    a owl:Restriction ;
    owl:onProperty schema:itemListElement ;
    owl:someValuesFrom schema:CreativeWork
  ] ;
  rdfs:isDefinedBy <gdx:> ;
  rdfs:label "Research Repository Service"@en-US ;
  rdfs:comment "A catalog of research resources made accessible by this services. These resources should be CreativeWorks such as schema:DataCatalog, schema:Dataset, schema:SoftwareApplications, schema:WebAPI, etc."@en-US .

<gdx:SearchService>
  a owl:namedIndividual, schema:ServiceChannel ;
  rdfs:isDefinedBy <gdx:> ;
  rdfs:label "Search Service Channel"@en-US ;
  rdfs:comment "A service provided for searching the resource catalog."@en-US .

<gdx:SubmissionService>
  a owl:namedIndividual, schema:ServiceChannel ;
  rdfs:isDefinedBy <gdx:> ;
  rdfs:label "Submssions Service Channel"@en-US ;
  rdfs:comment "A service provided for submitting resources to the catalog."@en-US .

<gdx:SyndicationService>
  a owl:namedIndividual, schema:ServiceChannel ;
  rdfs:isDefinedBy <gdx:> ;
  rdfs:label "Syndication Service Channel"@en-US ;
  rdfs:comment "A service provided for syndicating resources from the catalog."@en-US .

<gdx:Protocol-Access>
  a owl:namedIndividual, schema:DigitalDocument ;
  rdfs:isDefinedBy <gdx:> ;
  rdfs:label "Access Protocol"@en-US ;
  rdfs:comment "An access regulation."@en-US .

<gdx:Protocol-PreservationPolicy>
  a owl:namedIndividual, schema:DigitalDocument ;
  rdfs:isDefinedBy <gdx:> ;
  rdfs:label "Preservation Policy"@en-US ;
  rdfs:comment "A policy describing a preservation protocol."@en-US .

<gdx:Protocol-ResourceSubmissionPolicy>
  a owl:namedIndividual, schema:DigitalDocument ;
  rdfs:isDefinedBy <gdx:> ;
  rdfs:label "Resource Submission Policy"@en-US ;
  rdfs:comment "A policy describing the protocols for submitting resources to the repository."@en-US .

<gdx:Protocol-TermsOfUse>
  a owl:namedIndividual, schema:DigitalDocument ;
  rdfs:isDefinedBy <gdx:> ;
  rdfs:label "Terms of Use"@en-US ;
  rdfs:comment "A policy describing the Terms of Use."@en-US .

<gdx:Protocol-License>
  a owl:namedIndividual, schema:DigitalDocument ;
  rdfs:isDefinedBy <gdx:> ;
  rdfs:label "License"@en-US ;
  rdfs:comment "An applicable license."@en-US .

<gdx:SitemapXML>
  a owl:namedIndividual, schema:DigitalDocument ;
  rdfs:isDefinedBy <gdx:> ;
  rdfs:label "Sitemap XML File"@en-US ;
  rdfs:comment "A sitemap.xml file for a website that exposes URLs that should be indexed by a search engine harvester. A sitemap.xml file is one way to provide access to all resources offered by the gdx:ResearchResourceCatalog."@en-US .
